Complexitylib/Classes/PCP/Internal/AlgLevel.lean
@@ -4,7 +4,6 @@ Released under Apache 2.0 license as described in the file LICENSE.
 Authors: Bolton Bailey
 -/
 module
-public import Complexitylib.Classes.PCP.Internal.TowerFin
 public import Complexitylib.Classes.PCP.Internal.Materialize
 
 /-!
